wip about to reaname fInside -> fStrictlyInside

BISHOP.dfy
@@ -2,6 +2,119 @@
 include "Ownership-Parallel.dfy"
 include "Context.dfy"
 
+
+predicate enclosedBy(part : Object, whole : Object)
+  requires part.Ready()
+  requires whole.Ready()
+{
+   && (part.AMFO >= whole.AMFO)
+   && (forall p <- part.AMFO  :: (p in whole.AMFO) || (p.AMFO >= whole.AMFO))
+}
+
+predicate enclosedBy1(part : Object, whole : Object)
+  requires part.Ready()
+  requires whole.Ready()
+{
+    inside(part, whole) &&
+    forall p <- part.AMFO  :: (p in whole.AMFO) || (p.AMFO >= whole.AMFO)
+}
+
+predicate recEnclosedBy(part : Object, whole : Object)
+     requires part.Ready()
+    decreases part.AMFO
+{
+  || (part == whole)
+  || (forall x <- part.owner :: recEnclosedBy(x,whole))
+}
+
+lemma Enclosed_Enclosed(part : Object, whole : Object)
+  requires part.Ready()
+  requires whole.Ready()
+   ensures enclosedBy(part,whole) == recEnclosedBy(part,whole)
+   {
+    if (part == whole)
+      {
+        assert enclosedBy(part,whole) == recEnclosedBy(part,whole);
+        return;
+      }
+    forall x <- part.owner ensures (enclosedBy(x,whole) == recEnclosedBy(x,whole) ) //by
+      {
+
+      }
+
+   }
+
+
+
+lemma HappyFamilies(soup : set<Object>, whole : Object, ins: set<Object>, outs: set<Object>, sides: set<Object>)
+  requires ins   == allInside(soup, whole)
+  requires outs  == allOutside(soup, whole)
+  requires sides == allOffside(soup, whole)
+   ensures soup  == ins + outs + sides
+{}
+
+predicate Xoffside(part : Object, whole : Object) reads {} { not(colinear(part.AMFO,whole.AMFO)) }
+
+
+
+lemma prattt(part : Object)
+  requires part.Ready()
+   ensures forall x <- part.AMFO :: x in part.AMFO
+{}
+
+lemma SLICE_X_DICE(a : Object, amfo : OWNR, pivot : Object, below : OWNR, above : OWNR, aside : Owner)
+    //give that below == amfo - pivot.AMFO,
+    //then below + pivot.AMFO == amfo
+    requires a.Ready()
+    requires amfo == a.AMFO
+ requires AllReady(amfo)
+ requires pivot.Ready()
+ requires AllReady(below)
+ requires AllReady(above)
+ requires AllReady(aside)
+  ensures isFlat(amfo)
+ requires amfo > pivot.AMFO
+  ensures strictlyInside(a,pivot)
+//nope requires forall x <- below :: x.AMFO > pivot.AMFO    //stops ""side loadung"""
+//  requires below == amfo - pivot.AMFO
+  requires below == (set x <- amfo | strictlyInside(x,pivot))
+  requires above == (set x <- amfo | inside(pivot,x))
+  requires aside == amfo - (above + below)
+   ensures aside == (set x <- amfo | not(strictlyInside(x,pivot)) && not(inside(pivot,x)))
+   ensures aside == (set x <- amfo | not(strictlyInside(x,pivot) || inside(pivot,x)))
+   ensures aside == (set x <- amfo | not(inside(x,pivot) || inside(pivot,x)))
+   ensures aside == (set x <- amfo | not(colinear(x.AMFO, pivot.AMFO)))
+   ensures aside == (set x <- amfo | offside(x, pivot))
+
+
+   ensures below !! above !! aside
+
+   ensures amfo == below + above + aside
+
+    //  ensures pivot.AMFO == (set x <- amfo | not(strictlyInside(x,pivot)))
+//   ensures above <= pivot.AMFO
+////   ensures above >= pivot.AMFO
+  //  ensures below + pivot.AMFO == amfo
+  //  ensures amfo == pivot.AMFO + below
+  //  ensures forall x <- below :: (x in amfo) //&& (strictlyInside(x, pivot))
+  //  ensures forall x <- below :: x !in pivot.AMFO
+  // //nope ensures forall x <- below :: (strictlyInside(x, pivot))
+  //  ensures below >= (set x <- amfo | strictlyInside(x, pivot))
+  // //nope ensures below <= (set x <- amfo | strictlyInside(x, pivot))
+  {}
+
+
+
+
+
+
+
+
+
+
+
+
+
 lemma WhyDoesntThisWork(o : Object, pivot : Object, remainder : Owner)
   requires o.Ready()
   requires pivot.Ready()
@@ -30,7 +143,7 @@ lemma WhyDoesntThisWork(o : Object, pivot : Object, remainder : Owner)
 
    ensures forall r <- remainder :: (r.AMFO > pivot.AMFO)
 
-  ensures forall x <- o.AMFO, p <- pivot.AMFO ::
+///  ensures forall x <- o.AMFO, p <- pivot.AMFO ::  ????
 
     ensures forall x <- o.AMFO :: (x in remainder) == (x !in pivot.AMFO)
    //    ensures remainder == (set x <- o.AMFO | x.AMFO !in pivot.AMFO)
